src/ops.v
@@ -1,0 +1,33 @@
+Module Logical.
+Module Op.
+
+Class not_of int := not_op : int -> int.
+Class or_of int := or_op : int -> int -> int.
+Class and_of int := and_op : int -> int -> int.
+Class xor_of int := xor_op : int -> int -> int.
+Class shl_of int := shl_op : int -> int -> int.
+Class shr_of int := shr_op : int -> int -> int.
+
+End Op.
+End Logical.
+
+Import Logical.Op.
+
+Typeclasses Transparent not_of or_of and_of xor_of shl_of shr_of.
+
+Notation "~%C"    := not_op.
+Notation "~ x"    := (not_op x)     : computable_scope.
+Notation "||%C"   := or_op.
+Notation "x || y" := (or_op x y)   : computable_scope.
+Notation "&&%C"   := and_op.
+Notation "x && y" := (and_op x y)   : computable_scope.
+Notation "^^%C"    := xor_op.
+Notation "x ^^ y"  := (xor_op x y)
+ (at level 30, right associativity) : computable_scope.
+Notation ">>%C"    := shr_op.
+Notation "x >> y"  := (shr_op x y) 
+ (at level 30, right associativity) : computable_scope.
+Notation "<<%C"    := shl_op.
+Notation "x << y"  := (shl_op x y) 
+ (at level 30, right associativity) : computable_scope.
+
